working towards a proof that an infinite loop is an infinite loop.
- i should pull in paco to do the simulation proofs.
- the refactoring may not be ideal

theories/Eff.v
@@ -1,55 +1,147 @@
-Section freeD.
+Section Eff.
   Variable eff : Type -> Type.
 
-  CoInductive freeD (T : Type) : Type :=
-  | ret (_ : T)
-  | interact {A} (_ : eff A) (_ : A -> freeD T)
-  | delay (_ : freeD T).
+  Inductive EffF (Eff : Type) (T : Type) : Type :=
+  | retF (_ : T)
+  | interactF {A} (_ : eff A) (_ : A -> Eff)
+  | delayF (_ : Eff).
 
-  Arguments ret {_} _.
-  Arguments interact {_ _} _ _.
-  Arguments delay {_}.
+  Arguments retF {_ _} _.
+  Arguments interactF {_ _ _} _ _.
+  Arguments delayF {_ _} _.
+
+  CoInductive Eff (T : Type) : Type :=
+  | do (_ : EffF (Eff T) T).
+
+  Arguments do {_} _.
+
+  Definition getEff {T} (x : Eff T) : EffF (Eff T) T :=
+    match x with
+    | do y => y
+    end.
+
+  Definition ret {T} (x : T) : Eff T :=
+    do (retF x).
+
+  Definition interact {T U} (x : eff T) (k : T -> Eff U) : Eff U :=
+    do (interactF x k).
+
+  Definition delay {T} (x : Eff T)  : Eff T :=
+    do (delayF x).
+
+  Theorem getEff_eq : forall {T} (x : Eff T),
+      x = match getEff x with
+          | retF v => ret v
+          | interactF e k => interact e k
+          | delayF k => delay k
+          end.
+  Proof.
+    destruct x; destruct e; reflexivity.
+  Defined.
 
   Section bind.
-    Context {A B : Type} (k : A -> freeD B).
+    Context {A B : Type} (k : A -> Eff B).
 
-    CoFixpoint bind' (f : freeD A) : freeD B :=
-      match f with
-      | ret x => k x
-      | interact io k' => interact io (fun x => bind' (k' x))
-      | delay f => delay (bind' f)
+    CoFixpoint bind' (f : Eff A) : Eff B :=
+      match getEff f with
+      | retF x => k x
+      | interactF io k' => interact io (fun x => bind' (k' x))
+      | delayF f => delay (bind' f)
       end.
   End bind.
 
-  Definition bind {A B} (f : freeD A) (k : A -> freeD B) : freeD B :=
+  Definition bind {A B} (f : Eff A) (k : A -> Eff B) : Eff B :=
     bind' k f.
 
   (* I should use paco to define this *)
-  CoInductive freeD_eq {T} : freeD T -> freeD T -> Prop :=
-  | eq_ret : forall t, freeD_eq (ret t) (ret t)
+  CoInductive Eff_eq {T} : Eff T -> Eff T -> Prop :=
+  | eq_ret : forall t, Eff_eq (ret t) (ret t)
   | eq_interact : forall a (e : eff a) k1 k2,
-      (forall x, freeD_eq (k1 x) (k2 x)) ->
-      freeD_eq (interact e k1) (interact e k2)
-  | eq_delay : forall a b, freeD_eq a b ->
-                      freeD_eq (delay a) (delay b).
+      (forall x, Eff_eq (k1 x) (k2 x)) ->
+      Eff_eq (interact e k1) (interact e k2)
+  | eq_delay : forall a b, Eff_eq a b ->
+                      Eff_eq (delay a) (delay b).
 
-  CoInductive freeD_sim {T} : freeD T -> freeD T -> Prop :=
-  | sim_ret : forall t, freeD_sim (ret t) (ret t)
+  CoInductive Eff_sim {T} : Eff T -> Eff T -> Prop :=
+  | sim_ret : forall t, Eff_sim (ret t) (ret t)
   | sim_interact : forall a (e : eff a) k1 k2,
-      (forall x, freeD_sim (k1 x) (k2 x)) ->
-      freeD_sim (interact e k1) (interact e k2)
-  | sim_delay : forall a b, freeD_sim a b ->
-                       freeD_sim (delay a) (delay b).
+      (forall x, Eff_sim (k1 x) (k2 x)) ->
+      Eff_sim (interact e k1) (interact e k2)
+  | sim_delay : forall a b, Eff_sim a b ->
+                       Eff_sim (delay a) (delay b).
 
-End freeD.
+End Eff.
 
 
 Arguments bind {_ _ _} _ _.
 Arguments bind' {_ _ _} _ _.
+Arguments interactF {_ _ _ _} _ _.
 Arguments interact {_ _ _} _ _.
+Arguments retF {_ _ _} _.
 Arguments ret {_ _} _.
+Arguments delayF {_ _ _} _.
 Arguments delay {_ _} _.
+Arguments getEff {_ _} _.
 
+(** Interpretation of effects *)
+
+Section interp.
+
+  Context {eff eff' : Type -> Type}.
+
+  Variable do : forall {T}, eff T -> Eff eff' T.
+
+  CoFixpoint interp {T} (c : Eff eff T) : Eff eff' T :=
+    match getEff c with
+    | retF x => ret x
+    | interactF e k =>
+      match getEff (do _ e) with
+      | retF v => delay (interp (k v))
+      | interactF e k' =>
+        interact e (fun x => bind (k' x) (fun y => interp (k y)))
+      | delayF v => delay (@bind' _ _ _ (fun x => interp (k x)) v)
+      end
+    | delayF x => delay (interp x)
+    end.
+
+
+
+  Lemma interp_ret : forall {T} (v : T),
+      interp (ret v) = ret v.
+  Proof.
+    intros.
+    rewrite getEff_eq.
+    rewrite (getEff_eq _ (interp (ret v))).
+    reflexivity.
+  Defined.
+
+  (* This doesn't preserve stuttering *)
+  Lemma interp_interact : forall {a b} (e : eff a) (k : a -> Eff eff b),
+      interp (interact e k) =
+      bind (do _ e) (fun x => interp (k x)).
+  Proof.
+    intros.
+    rewrite getEff_eq. symmetry. rewrite getEff_eq. symmetry.
+    simpl.
+    destruct (getEff (do a e)); simpl.
+    { admit. }
+    { reflexivity. }
+    { reflexivity. }
+  Admitted.
+
+  Lemma interp_delay : forall {a} (k : Eff eff a),
+      interp (delay k) = delay (interp k).
+  Proof.
+    intros.
+    rewrite getEff_eq. symmetry. rewrite getEff_eq. symmetry.
+    reflexivity.
+  Defined.
+
+End interp.
+
+(** Effects **)
+
+(* union of effects *)
 Section bothE.
   Context {f g : Type -> Type}.
   Inductive both (T : Type) : Type :=
@@ -61,23 +153,22 @@ Arguments both _ _ _ : clear implicits.
 Arguments bleft {_ _ _} _.
 Arguments bright {_ _ _} _.
 
-
 Section inj.
 
   Variable eff eff' : Type -> Type.
 
-  CoFixpoint injL {T} (c : freeD eff T) : freeD (both eff eff') T :=
-    match c with
-    | ret x => ret x
-    | interact e k => interact (bleft e) (fun x => injL (k x))
-    | delay x => delay (injL x)
+  CoFixpoint injL {T} (c : Eff eff T) : Eff (both eff eff') T :=
+    match getEff c with
+    | retF x => ret x
+    | interactF e k => interact (bleft e) (fun x => injL (k x))
+    | delayF x => delay (injL x)
     end.
 
-  CoFixpoint injR {T} (c : freeD eff' T) : freeD (both eff eff') T :=
-    match c with
-    | ret x => ret x
-    | interact e k => interact (bright e) (fun x => injR (k x))
-    | delay x => delay (injR x)
+  CoFixpoint injR {T} (c : Eff eff' T) : Eff (both eff eff') T :=
+    match getEff c with
+    | retF x => ret x
+    | interactF e k => interact (bright e) (fun x => injR (k x))
+    | delayF x => delay (injR x)
     end.
 
 End inj.
@@ -85,27 +176,7 @@ End inj.
 Arguments injL {_} _ {_} _.
 Arguments injR {_ _} _ _.
 
-Section interp.
-
-  Context {eff eff' : Type -> Type}.
-
-  Variable do : forall {T}, eff T -> freeD eff' T.
-
-  CoFixpoint interp {T} (c : freeD eff T) : freeD eff' T :=
-    match c with
-    | ret x => ret x
-    | interact e k =>
-      match do _ e with
-      | ret v => delay (interp (k v))
-      | interact e k' =>
-        interact e (fun x => bind (k' x) (fun y => interp (k y)))
-      | delay v => delay (@bind' _ _ _ (fun x => interp (k x)) v)
-      end
-    | delay x => delay (interp x)
-    end.
-End interp.
-
-
+(* the fixpoint effect *)
 Section Fix.
 
   Variable a : Type.
@@ -118,27 +189,27 @@ Section Fix.
   (** Begin a bunch of variants to try to implement mfix *)
 
   Section mfix.
-    Variable f : freeD (both eff fixpoint) a.
+    Variable f : Eff (both eff fixpoint) a.
 
     CoFixpoint finterp_then
-           {T b : Type} (k' : T -> freeD eff b)
-               (c : freeD (both eff fixpoint) T) : freeD eff b :=
-      match c with
-      | ret x => delay (k' x)
-      | interact (bleft e) k =>
+           {T b : Type} (k' : T -> Eff eff b)
+               (c : Eff (both eff fixpoint) T) : Eff eff b :=
+      match getEff c with
+      | retF x => delay (k' x)
+      | interactF (bleft e) k =>
         interact e (fun x => finterp_then k' (k x))
-      | interact (bright e) k =>
+      | interactF (bright e) k =>
         delay (finterp_then k' (bind' (fun x => k match e with
                                         | rec => x
                                         end) f))
-      | delay x => delay (finterp_then k' x)
+      | delayF x => delay (finterp_then k' x)
       end.
 
-    Definition mfix : freeD eff a := finterp_then ret f.
+    Definition mfix : Eff eff a := finterp_then ret f.
   End mfix.
 
-  Definition go (mfix : freeD eff a)
-    T (X : both eff fixpoint T) : freeD eff T :=
+  Definition go (mfix : Eff eff a)
+    T (X : both eff fixpoint T) : Eff eff T :=
     match X with
     | bleft e => interact e ret
     | bright f0 =>
@@ -151,10 +222,14 @@ Section Fix.
       mfix f = interp (go (mfix f)) f.
   Proof. Admitted.
 
+  Theorem mfix_ret : forall v, mfix (ret v) = ret v.
+  Proof. Admitted.
+
 End Fix.
 
 Arguments mfix {_} _.
 
+(* the state effect *)
 Section stateE.
   Variable s : Type.
   Inductive state : Type -> Type :=
@@ -166,17 +241,41 @@ End stateE.
 Arguments Get {_}.
 Arguments Put {_} _.
 
+(* the empty effect *)
 Section nothingE.
   Inductive nothing : Type -> Type := .
 End nothingE.
 
 (** Testing *)
-Definition trial : freeD nothing False :=
+Definition trial : Eff nothing False :=
   mfix nothing (interact (bright (rec False)) ret).
 
+Section diverge.
+  Context {eff : Type -> Type}.
+  Variable t : Type.
+  CoFixpoint diverge : Eff eff t :=
+    delay diverge.
 
+  Theorem diverge_eq : diverge = delay diverge.
+  Proof. symmetry. rewrite getEff_eq. reflexivity. Defined.
 
-Goal freeD_eq _ trial (cofix rec := delay rec).
+End diverge.
+
+Require Import Setoid.
+
+Goal Eff_eq _ trial (diverge _).
   cofix rec.
-  unfold trial. rewrite mfix_unfold.
+  unfold trial.
+  rewrite mfix_unfold.
+  rewrite interp_interact. simpl go.
+  rewrite mfix_unfold. rewrite interp_interact.
+  Eval compute in fun f => getEff (mfix nothing f ret).
+
+  rewrite (getEff_eq _ (interp (go _ _ _) _)).
+
+
+  simpl.
+  rewrite (getEff_eq _ (diverge False)). simpl.
+
+
 Admitted.
